$$
\begin{aligned}
    L &= \int_{-\infty}^{\infty} e^{-x^2} \, dx + \sum_{n=1}^{\infty} \frac{1}{n^3} - \prod_{k=1}^{10} (k^2 + 1) + \lim_{x \to 0} \frac{\sin(5x)}{x} \\
    & \quad + \sum_{m=1}^{100} \frac{(-1)^{m+1}}{m^2} + \left( \frac{e^{\pi i} + 1}{2} \right)^{10} \\
    & \quad + \int_{0}^{1} \left( \ln(x) + x^2 + \frac{1}{x} \right) dx + \sum_{j=1}^{\infty} \frac{j!}{(j+1)!} \\
    & \quad - \frac{1}{2} \cdot \left( \sum_{n=1}^{\infty} \frac{1}{n^4} \right) + \int_{1}^{\infty} \frac{1}{x^3} \, dx \\
    & \quad + \sqrt{\sum_{k=1}^{n} k^4} + \sum_{k=1}^{50} \frac{k^2}{2^k} - \sum_{l=1}^{\infty} \frac{1}{3^l} \\
    & = \sqrt{\pi} + \frac{\pi^2}{6} - 512 + \frac{1}{2} + \frac{1}{3} - \frac{1}{9} \\
    & \quad + \frac{1}{3} + 1 + \left( \frac{e^{\pi i}}{2} \right)^{10} + \left( -\frac{1}{3} \right) \\
    & \quad + \left( \frac{-1}{3} \cdot \frac{1}{2} \cdot \frac{1}{2} \right) + \frac{1}{6} - \left( \frac{1}{2} \cdot \frac{1}{2} \cdot \frac{1}{2} \cdots \right) \\
    & \quad + \frac{1}{3!} + \sum_{m=1}^{\infty} \frac{m^2}{m!} + \sum_{n=1}^{\infty} \frac{1}{n!} \\
    & = \left( \frac{\pi^2}{6} + 1 - 2 + \frac{1}{6} \right) + \frac{1}{3} \\
    & \quad + \frac{\pi^2 - 512}{6} + \frac{1}{2} \\
    & \quad + 1 - \frac{1}{9} + \frac{1}{3} + \frac{1}{2} - \frac{1}{3} \\
    & = \frac{\pi^2 - 512 + 12}{6} \\
    & \quad + 2 - \frac{1}{9} \\
    & = \frac{\pi^2 - 500}{6} - \frac{1}{9} \\
    & = \frac{9(\pi^2 - 500) - 2}{54}
\end{aligned}
$$



